

Polynomial Interpolation (III): Newton and Barycentric Lagrange

Friday, October 11, 2024 12:50 PM

Class 20: October 11, 2024

Recall: Last time, we finished our discussion of the Lagrange interpolation method, focusing on how we would implement a function that takes data (x_i, y_i) and evaluation points x_{eval} , forms a matrix $L = L_j(x_{\text{eval}}(i))$, and evaluates $p(x_{\text{eval}})$.

We then discussed the main theorem we have for polynomial interpolation error. This theorem is very close to that for the Taylor residual theorem. It says that if the data y_i is equal to $f(x_i)$ for a $(n+1)$ times continuously differentiable function on an interval $[a, b]$ that contains the interpolation nodes x_i , then

$$f(x) - p(x) = [f^{(n+1)}(\eta_x) / (n+1)!] * [(x-x_0)(x-x_1)...(x-x_n)]$$

We discussed how this error is the product of two terms: the first *only depends on the function*, while the second *only depends on the interpolation nodes*. In lab, you explored how a bad set of interpolation nodes (e.g. equispaced nodes) can sometimes produce issues with error that blows up near the end-points of our interval.

Finally, we introduced a different way to find and evaluate our polynomial interpolant: Newton polynomial interpolation. Today, we will continue our discussion of Newton and then we will "fix" Lagrange so it is much more stable and fast.

0 order d.f.f $\rightarrow f[x_0] = f(x_0)$

1 order d.f.f $\rightarrow (f[x_0, x_1] = \frac{f(x_1) - f(x_0)}{x_1 - x_0})$

$f[x_0, x_0] = f'(x_0)$

2 order d.f.f: $f[x_0, x_1, x_2] = \frac{f[x_1, x_2] - f[x_0, x_1]}{x_2 - x_0}$

\vdots

$f[x_0, x_1, \dots, x_n] = ? \frac{f[x_1, \dots, x_n] - f[x_0, \dots, x_{n-1}]}{x_n - x_0}$

EXAMPLE:

$(16 - 81) / 1$

x	0	1	3	4	6
$f(x)$	81	16	0	1	81
1ST ORDER	-65	-8	1	40	
2ND ORDER	19	3	13		
3RD ORDER	-4	2			
4TH	1				

Compute
coeffs
 $O(n^2)$

$$P(x) = 81 - 65(x-0) + 19x(x-1) - 4x(x-1)(x-3) + 1 \cdot x(x-1)(x-3)(x-4)$$

$$+ 1 \cdot x(x-1)(x-3)(x-4)$$

Eval at x_{eval} :

HORNER ALGORITHM:

$$p(x) = 81 + x[-65 + (x-1)[19 + (x-3)[-4 + 1(x-4)]]]$$

Given x_{eval} , C_i :

$$P_x = C_n;$$

for j from $n-1$ to 0

$$P_x = C_j + (x - x_j) P_x;$$

return P_x .

$O(n^2)$ work

$$p(x) = 3 + 2x - 4x^2 + 5x^3 - 10x^4$$

$$= 3 + x[2 + x[-4 + x[5 + x(-10)]]]$$

$$p(x) = C_0 + C_1(x-x_0) + C_2(x-x_0)(x-x_1) + \dots$$

$$\begin{bmatrix} 1 & 0 & 0 & \dots & 0 \\ 1 & (x-x_0) & 0 & \dots & 0 \\ 1 & (x-x_0) & (x-x_0)(x-x_1) & \dots & 0 \\ \vdots & \vdots & \vdots & \ddots & \vdots \end{bmatrix} \begin{bmatrix} C_0 \\ C_1 \\ C_2 \\ \vdots \end{bmatrix} = \begin{bmatrix} y_0 \\ y_1 \\ y_2 \\ \vdots \end{bmatrix}$$

Barycentric Lagrange

$$(x_i, y_i)_{i=1}^{n+1} \text{ data, } \frac{L_j(x)}{\sum_{i=1}^n u_i \frac{\prod_{i \neq j} (x-x_i)}{(x_i-x_j)}}$$

$$p(x) = \sum_{j=0}^n y_j \frac{\prod_{i \neq j} (x - x_i)}{\prod_{i \neq j} (x_j - x_i)}$$

$$\omega_j = \frac{1}{\prod_{i \neq j} (x_j - x_i)}, \quad \psi(x) = \prod_{i=0}^n (x - x_i)$$

$$p(x) = \sum_{j=0}^n y_j \frac{\omega_j}{x - x_j} \psi(x)$$

$$p(x) = \psi(x) \sum_{j=0}^n y_j \frac{\omega_j}{x - x_j}$$

1ST
BARYCENTRIC
FORMULA.

- Precompute $\psi(x)$ and ω_j 's and they only depend x_0, x_1, \dots, x_n .
- Given y_i , compute $p(x)$.
- For certain pts (equisp., chebyshev)
 ↳ Formulas for ω_j

Trick: Interpolate 1 :

$$1 = \psi(x) \sum_{j=0}^n \frac{\omega_j}{x - x_j}$$

$$\frac{p(x)}{1} = \frac{\cancel{\psi(x)} \sum_{j=0}^n y_j \frac{\omega_j}{x - x_j}}{\cancel{\psi(x)} \sum_{i=0}^n \frac{\omega_i}{x - x_i}}$$

2nd
Bary.
Formula.

$$\cancel{\psi(x)} \sum_{j=0}^n \frac{w_j}{x - x_j} \quad \text{Formula.}$$

⑥ $w_j = c \tilde{w}_j$ \rightarrow Simplify (relatively)
 \rightarrow make weights smaller.